bin/prelude.bpl
@@ -3,21 +3,34 @@ type ref;
 type name;
 type ptr;
 const unique null:ref;
-function Ptr(ref, int) returns (ptr);
+function Ptr(ref, bv32) returns (ptr);
 function Obj(ptr) returns (ref);
-function Off(ptr) returns (int);
+function Off(ptr) returns (bv32);
 
 // Ptr, Obj, Off axioms
 axiom(forall x:ptr :: {Obj(x)}{Off(x)} x == Ptr(Obj(x), Off(x)));
-axiom(forall x_obj:ref, x_off:int :: {Ptr(x_obj, x_off)} x_obj == Obj(Ptr(x_obj, x_off)));
-axiom(forall x_obj:ref, x_off:int :: {Ptr(x_obj, x_off)} x_off == Off(Ptr(x_obj, x_off)));
+axiom(forall x_obj:ref, x_off:bv32 :: {Ptr(x_obj, x_off)} x_obj == Obj(Ptr(x_obj, x_off)));
+axiom(forall x_obj:ref, x_off:bv32 :: {Ptr(x_obj, x_off)} x_off == Off(Ptr(x_obj, x_off)));
+
+function {:bvbuiltin "bvadd"} add(p1:bv32, p2:bv32) returns (bv32);
+function {:bvbuiltin "bvsub"} sub(p1:bv32, p2:bv32) returns (bv32);
+function {:bvbuiltin "bvmul"} mul(p1:bv32, p2:bv32) returns (bv32);
+function {:bvbuiltin "bvult"} ult(p1:bv32, p2:bv32) returns (bool);
+function {:bvbuiltin "bvugt"} ugt(p1:bv32, p2:bv32) returns (bool);
+function {:bvbuiltin "bvule"} ule(p1:bv32, p2:bv32) returns (bool);
+function {:bvbuiltin "bvuge"} uge(p1:bv32, p2:bv32) returns (bool);
+function {:bvbuiltin "bvslt"} slt(p1:bv32, p2:bv32) returns (bool);
+function {:bvbuiltin "bvsgt"} sgt(p1:bv32, p2:bv32) returns (bool);
+function {:bvbuiltin "bvsle"} sle(p1:bv32, p2:bv32) returns (bool);
+function {:bvbuiltin "bvsge"} sge(p1:bv32, p2:bv32) returns (bool);
+
 
 // Mutable
 var Mem:[ptr]ptr;
 var Alloc:[ref]name;
 
 // Immutable
-function Size(ref) returns (int);
+function Size(ref) returns (bv32);
 
 // Undefined ptr value
 var undef:ptr;
@@ -27,18 +40,18 @@ const unique UNALLOCATED:name;
 const unique ALLOCATED:name;
 
 
-procedure __SMACK_alloca(obj_size:int) returns (new:ptr);
+procedure __SMACK_alloca(obj_size:bv32) returns (new:ptr);
 modifies Alloc;
 ensures old(Alloc)[Obj(new)] == UNALLOCATED && Alloc[Obj(new)] == ALLOCATED;
-ensures Off(new) == 0;
+ensures Off(new) == 0bv32;
 ensures Obj(new) != null;
 ensures Size(Obj(new)) == obj_size;
 ensures (forall x_obj:ref :: {Alloc[x_obj]} x_obj == Obj(new) || old(Alloc)[x_obj] == Alloc[x_obj]);
 
-procedure __SMACK_malloc(obj_size:int) returns (new:ptr);
+procedure __SMACK_malloc(obj_size:bv32) returns (new:ptr);
 modifies Alloc;
 ensures old(Alloc)[Obj(new)] == UNALLOCATED && Alloc[Obj(new)] == ALLOCATED;
-ensures Off(new) == 0;
+ensures Off(new) == 0bv32;
 ensures Obj(new) != null;
 ensures Size(Obj(new)) == obj_size;
 ensures (forall x_obj:ref :: {Alloc[x_obj]} x_obj == Obj(new) || old(Alloc)[x_obj] == Alloc[x_obj]);
@@ -46,7 +59,7 @@ ensures (forall x_obj:ref :: {Alloc[x_obj]} x_obj == Obj(new) || old(Alloc)[x_ob
 procedure __SMACK_free(pointer:ptr);
 modifies Alloc;
 requires Alloc[Obj(pointer)] == ALLOCATED;
-requires Off(pointer) == 0;
+requires Off(pointer) == 0bv32;
 ensures Alloc[Obj(pointer)] != UNALLOCATED;
 ensures (forall x:ref :: {Alloc[x]} Obj(pointer) == x || old(Alloc)[x] == Alloc[x]);
 
@@ -59,34 +72,34 @@ procedure __SMACK_Proc_ICMP_NE(a:ptr, b:ptr) returns (result:bool);
 ensures result == (a != b);
 
 procedure __SMACK_Proc_ICMP_SGE(a:ptr, b:ptr) returns (result:bool);
-ensures result == (Off(a) >= Off(b));
+ensures result == sge(Off(a), Off(b));
 procedure __SMACK_Proc_ICMP_UGE(a:ptr, b:ptr) returns (result:bool);
-ensures result == (Off(a) >= Off(b));
+ensures result == uge(Off(a), Off(b));
 
 procedure __SMACK_Proc_ICMP_SLE(a:ptr, b:ptr) returns (result:bool);
-ensures result == (Off(a) <= Off(b));
+ensures result == sle(Off(a), Off(b));
 procedure __SMACK_Proc_ICMP_ULE(a:ptr, b:ptr) returns (result:bool);
-ensures result == (Off(a) <= Off(b));
+ensures result == ule(Off(a), Off(b));
 
 procedure __SMACK_Proc_ICMP_SLT(a:ptr, b:ptr) returns (result:bool);
-ensures result == (Off(a) < Off(b));
+ensures result == slt(Off(a), Off(b));
 procedure __SMACK_Proc_ICMP_ULT(a:ptr, b:ptr) returns (result:bool);
-ensures result == (Off(a) < Off(b));
+ensures result == ult(Off(a), Off(b));
 
 procedure __SMACK_Proc_ICMP_SGT(a:ptr, b:ptr) returns (result:bool);
-ensures result == (Off(a) > Off(b));
+ensures result == sgt(Off(a), Off(b));
 procedure __SMACK_Proc_ICMP_UGT(a:ptr, b:ptr) returns (result:bool);
-ensures result == (Off(a) > Off(b));
+ensures result == ugt(Off(a), Off(b));
 
 
 procedure __SMACK_Add(a:ptr, b:ptr) returns (result:ptr);
-ensures Obj(result) == null && Off(result) == Off(a) + Off(b);
+ensures Obj(result) == null && Off(result) == add(Off(a), Off(b));
 
 procedure __SMACK_Sub(a:ptr, b:ptr) returns (result:ptr);
-ensures Obj(result) == null && Off(result) == Off(a) - Off(b);
+ensures Obj(result) == null && Off(result) == sub(Off(a), Off(b));
 
 procedure __SMACK_Mul(a:ptr, b:ptr) returns (result:ptr);
-ensures Obj(result) == null && Off(result) == Off(a) * Off(b);
+ensures Obj(result) == null && Off(result) == mul(Off(a), Off(b));
 
 procedure __SMACK_SDiv(a:ptr, b:ptr) returns (result:ptr);
 ensures Obj(result) == null;
@@ -122,16 +135,16 @@ procedure __SMACK_Trunc(a:ptr) returns (result:ptr);
 ensures result == a;
 
 
-function __SMACK_PtrArith(pointer:ptr, offset:int, size:int) returns (result:ptr);
-axiom(forall p:ptr, off:int, size:int :: {__SMACK_PtrArith(p, off, size)}
-  __SMACK_PtrArith(p, off, size) == Ptr(Obj(p), Off(p) + off * size));
+function __SMACK_PtrArith(pointer:ptr, offset:bv32, size:bv32) returns (result:ptr);
+axiom(forall p:ptr, off:bv32, size:bv32 :: {__SMACK_PtrArith(p, off, size)}
+  __SMACK_PtrArith(p, off, size) == Ptr(Obj(p), add(Off(p), mul(off, size))));
 
 procedure __SMACK_BoolToInt(a:bool) returns (result:ptr);
 ensures Obj(result) == null;
-ensures (a && Off(result) != 0) || (!a && Off(result) == 0);
+ensures (a && Off(result) != 0bv32) || (!a && Off(result) == 0bv32);
 
 procedure __SMACK_isInt(x:ptr) returns (result:ptr);
-ensures (Obj(x) == null && result != Ptr(null, 0)) || (Obj(x) != null && result == Ptr(null, 0));
+ensures (Obj(x) == null && result != Ptr(null, 0bv32)) || (Obj(x) != null && result == Ptr(null, 0bv32));
 
 procedure __SMACK_nondet() returns (x:ptr);
 
